{
 "cells": [
  {
   "cell_type": "markdown",
   "id": "b9b85b54",
   "metadata": {},
   "source": [
    "# A terminating, non-cyclic* path towards the Collatz conjecture\n",
    "\n",
    "Jon Seymour \\<a_beautiful_k\\@wildducktheories.com\\>\n",
    "\n",
    "14 October 2023\n",
    "\n",
    "## Abstract\n",
    "\n",
    "_\"Mathematics may not be ready for such problems\"_ - Paul Erdős on the Collatz conjecture.\n",
    "\n",
    "It has long been known that the following identity applies to all paths of the Collatz sequence.\n",
    "\n",
    "$2^nx_{n} - 3^{m}x_{0} = k$\n",
    "\n",
    "where $x_{0}$ is the initial term and $x_{n}$ is the final term and $n$, $m$ and $k$ are path dependent parameters.\n",
    "\n",
    "It is known that $n$ and $m$ are determined exactly by the number even and odd terms in the sequence (respectively) and $k$ is a constant but rarely, if ever, has a general formula for $k$ been presented in the literature.\n",
    "\n",
    "This seems strange given that if we want to know the truth of the Collatz conjecture, we want to show that for every $x_{0}$ there is a $k$ such that $2^n - 3^{m}x_{0} = k$\n",
    "\n",
    "One explanation may be that the known formula for k is so unweildy that it is regarded as ugly and of no practical use.\n",
    "\n",
    "Yet if lack of beauty is the reason, then this can hardly be the case because, as this paper shows, the formula for k is, in fact, an expression of this form:\n",
    "\n",
    "$k = 2^{e_{n-1}}x_{n}-3^{o_{n-1}}x_0=\\sum_{i=0}^{i=n-1}{{2^{p_{i}}3^{q_{i}}r_{i}}}$\n",
    "\n",
    "for some path dependent parameters $p_{i}, q_{i}, r_{i}$ and that these parameters are trivial to derive for any finite Collatz sequence.\n",
    "\n",
    "This is, in the authors' opinion, a rather beautiful identity and surely permits some deeper reasoning about the truth of the conjecture.\n",
    "\n",
    "This paper shows how to derive $p_{i}$, $q_{i}$ and $r_{i}$ and hence $k$ for all finite Collatz sequences.\n",
    "\n",
    "Furthermore, this identity was derived with nothing more than high school mathematics which, if the identity is not already known in the literature, would be remarkable given the statement by Paul Erdős given above.\n",
    "\n",
    "But, be very clear, this paper **does not contain a proof of the Collatz conjecture**. It may be an important stepping stone on a path towards the Collatz conjecture but it is not the final proof itself.\n",
    "\n",
    "## A useful recurrence relation\n",
    "\n",
    "This paper examines a recurrence relation of the form:\n",
    "\n",
    "$x_{n+1} = \\frac{x_n+m_n(5x_n+2)}{2}, m_n=x_n\\pmod{2}$\n",
    "\n",
    "This sequence is identical to the known Collatz sequence, more traditionally defined as:\n",
    "\n",
    "$x_{n+1} = 3x_n + 1, x\\equiv1\\pmod{2}$\n",
    "\n",
    "$x_{n+1} = \\frac{x_n}{2}, x\\equiv0\\pmod{2}$\n",
    "\n",
    "That the relation is equivalent to the Collatz sequence is evident by re-arranging and simplifying this equation:\n",
    "\n",
    "$x_{n+1} = m_n(3x_n+1)+(1-m_n)\\frac{x}{2}$\n",
    "\n",
    "## Alternative forms of the recurrence relation\n",
    "\n",
    "Using the identity: \n",
    "\n",
    "$5m+1 = 6^m = 2^m3^m \\iff {m}\\in\\{0,1\\}$ \n",
    "\n",
    "the same recurrence relation can also be expressed in all of the following ways:\n",
    "\n",
    "$x_{n+1} = \\frac{(5m_n+1)x_n+2m_n}{2}$\n",
    "\n",
    "$x_{n+1} = \\frac{6^{m_n}x_n+2m_n}{2}$\n",
    "\n",
    "$x_{n+1} = \\frac{2^{m_n}3^{m_n}x_n+2m_n}{2}$\n",
    "\n",
    "$x_{n+1} = \\frac{2^{m_n}(3^{m_n}x_n+1)}{2}$\n",
    "\n",
    "$x_{n+1} = 2^{{m_n}-1}(3^{m_n}x_n+1)$\n",
    "\n",
    "and, finally, this:\n",
    "\n",
    "$x_{n+1} = 2^{{m_n}-1}((2+1)^{m_n}x_n+1)$\n",
    "\n",
    "which has certain important properties which may be expanded upon in a future paper should ongoing research into these prove fruitful."
   ]
  },
  {
   "cell_type": "code",
   "execution_count": 1,
   "id": "085cafe5",
   "metadata": {},
   "outputs": [],
   "source": [
    "from fractions import Fraction\n",
    "import math\n",
    "\n",
    "def m(x):\n",
    "    return x%2\n",
    "\n",
    "def succ(x):\n",
    "    succ=(x+m(x)*(5*x+2))//2\n",
    "    assert not(x%2 == 0) or succ == x//2\n",
    "    assert not(x%2 == 1) or succ == 3*x+1\n",
    "    return succ\n",
    "\n",
    "def collatz(x0, n):\n",
    "    x=x0\n",
    "    for k in range(0, n):\n",
    "        yield {\"k\": k, \"x\": x, \"x0\": x0, \"m\": m(x), \"succ\": succ(x)}    \n",
    "        x=succ(x)\n",
    "\n",
    "result=[e for e in collatz(27, 10)]\n",
    "#result"
   ]
  },
  {
   "cell_type": "markdown",
   "id": "56c3b852",
   "metadata": {},
   "source": [
    "## The sequences $o_{n}$, $e_{n}$\n",
    "\n",
    "Let $o_{0} = m_0, o_{n+1} = o_{n}+m_{n+1}, n>0$.\n",
    "\n",
    "Let $e_{n} = {n+1}-o_{n}$\n",
    "\n",
    "Clearly:\n",
    "\n",
    "$o_{n} = \\sum_{k=0}^{k=n}{m_k}$\n",
    "\n",
    "$e_{n} = \\sum_{k=0}^{k=n}(1-{m_k})$\n",
    "\n",
    "### Interpretation\n",
    "\n",
    "The series $o_{n}$ and $e_{n}$ is that they represent the number of odd and even terms in the path between $x_0$ and $x_n$. "
   ]
  },
  {
   "cell_type": "code",
   "execution_count": 2,
   "id": "312562df",
   "metadata": {},
   "outputs": [],
   "source": [
    "def o(seq):\n",
    "    for e in seq:\n",
    "        if e[\"k\"] == 0:\n",
    "            e[\"o\"]=0\n",
    "        else:\n",
    "            e[\"o\"]=pred[\"o\"]+e[\"m\"]            \n",
    "        assert e[\"o\"] <= e[\"k\"]\n",
    "        yield e\n",
    "        pred=e\n",
    "\n",
    "result=[e for e in o(collatz(27, 10))]\n",
    "#result"
   ]
  },
  {
   "cell_type": "markdown",
   "id": "50c379c3",
   "metadata": {},
   "source": [
    "## An expression for $x_{n}$ in terms of $x_{0}$.\n",
    "\n",
    "### the sequences $a_{n}$, $c_{n}$ and $d_{n}$\n",
    "\n",
    "In this section we rewrite each term $x_{n}$ as combination of terms from\n",
    "three simpler monotonically incresing sequences: \n",
    "- $a_{n}$ (_the accumulator sequence_)\n",
    "- $c_{n}$ (_the coefficient sequence_)\n",
    "- $d_{n}$ (_the divisor sequence_).\n",
    "\n",
    "Let the first term of the sequence, $x_{n}$ be named $x_{0}$ with subsequent terms being $x_{1}, x_{2}$ et cetera.\n",
    "\n",
    "Then we can define:\n",
    "\n",
    "$x_{n}=\\frac{c_{0}x_{0}+a_{n}}{d_{n}}$\n",
    "\n",
    "with $a_{0}=0$, $c_{0}=1$ and $d_{0}=1$.\n",
    "\n",
    "Now, let's derive an expression for $x_{n+1}$ in terms of $x_{0}, a_{n}$ and $d_{n}$\n",
    "\n",
    "Recall that:\n",
    "\n",
    "$x_{n+1} = \\frac{x_n+m_n(5x_n+2)}{2}$\n",
    "\n",
    "Substituting $\\frac{c_{n}x_{n}+a_{n}}{d_{n}}$ for $x_n$ yields:\n",
    "\n",
    "$x_{n+1} = \\frac{\\frac{c_{n}x_{n}+a_{n}}{d_{n}}+m_n(5(\\frac{c_{n}x_{n}+a_{n}}{d_{n}})+2)}{2}$\n",
    "\n",
    "Simplifying:\n",
    "\n",
    "$x_{n+1} = \\frac{{c_{n}x_{n}+a_{n}}+m_n(5({c_{n}x_{n}+a_{n}})+2d_{n})}{2d_{n}}$\n",
    "\n",
    "Redistributing terms:\n",
    "\n",
    "$x_{n+1}=\\frac{{c_{n}(5m_{n}+1)x_{n}+a_{n}(5m_{n}+1)}+m_n2d_{n}}{2d_{n}}$\n",
    "\n",
    "Noting the identity:\n",
    "\n",
    "$5m_{n}+1 = 6^{m_n}$\n",
    "\n",
    "$a_n$ can be further simplified to:\n",
    "\n",
    "$x_{n+1}=\\frac{6^{m_n}{c_{n}x_{n}+6^{m_n}a_{n}}+m_n2d_{n}}{2d_{n}}$\n",
    "\n",
    "This is of the form:\n",
    "\n",
    "$x_{n+1}=\\frac{c_{n+1}x_{n+1}+a_{n+1}}{d_{n+1}}$\n",
    "\n",
    "with:\n",
    "\n",
    "$a_{n+1}=6^{m_n}a_{n}+m_{n}2d_{n}$\n",
    "\n",
    "$c_{n+1}=6^{m_n}c_{n}$\n",
    "\n",
    "$d_{n+1}=2d_{n}$\n",
    "\n",
    "## Rewriting $a_{n+1}$, $c_{n+1}$, $d_{n+1}$, $x_{n+1}$ in terms of $x_0$\n",
    "\n",
    "### Case: $x_0 \\rightarrow x_1$\n",
    "\n",
    "We can check this for n=0 as follows:\n",
    "\n",
    "$a_{1}=6^{m_0}a_{0}+2m_{0}d_{0}=2m_{0}d_{0}=2m_{0}$\n",
    "\n",
    "$c_{1}=6^{m_0}c_{0}=6^{m_0}$\n",
    "\n",
    "$d_{1}=2d_{0}=2$\n",
    "\n",
    "$x_{1}=\\frac{6^{m_0}x_{0}+2m_{0}}{2} = \\frac{({5m_{0}+2}){x_0}+m_{0}}{2} = \\frac{x_{0} + m_{0}(5x_{0}+2)}{2}$\n",
    "\n",
    "### Case: $x_0 \\rightarrow x_1 \\rightarrow x_2$\n",
    "\n",
    "$a_{2}=6^{m_1}a_{1}+2d_{1}m_{1} = 6^{m_1}m_{0}2+m_{1}4$\n",
    "\n",
    "$c_{2}=6^{m_1}c_{1}=6^{m_1}6^{m_0}$\n",
    "\n",
    "$d_{2}=2d_{1} = 4$\n",
    "\n",
    "$x_{2}=\\frac{6^{m_1}6^{m_0}x_{0}+6^{m_1}m_{0}2+m_{1}4}{4}$\n",
    "\n",
    "### Case: $x_0 \\rightarrow x_1 \\rightarrow x_2 \\rightarrow x_3$\n",
    "\n",
    "$a_{3}=6^{m_2}a_{2}+2d_{2}m_{2}=6^{m_2}(6^{m_1}2m_{0}+4m_{1})+m_{2}8=6^{m_2}6^{m_1}m_{0}2+6^{m_2}m_{1}4+m_{2}8$\n",
    "\n",
    "$a_{3} = 6^{o_2}(\\sum_{i=0}^{i=2}{\\frac{2^{i+1}m_{i}}{6^{o_i}}})$\n",
    "\n",
    "$c_{3}=6^{m_2}6^{m_1}6^{m_0}=6^{o_{2}}$\n",
    "\n",
    "$d_{3}=8=2^3$\n",
    "\n",
    "$x_{3}=\\frac{6^{o_{2}}x_0+6^{o_2}(\\sum_{i=0}^{i=2}{\\frac{2^{i+1}m_{i}}{6^{o_i}}})}{2^3}$\n",
    "\n",
    "$x_{3}=6^{o_{2}}(\\frac{x_0+\\sum_{i=0}^{i=2}{\\frac{2^{i+1}m_{i}}{6^{o_i}}})}{2^3})$\n",
    "\n",
    "### Case: $x_0 \\rightarrow \\ldots \\rightarrow x_n \\rightarrow x_{n+1}$\n",
    "\n",
    "It can be shown that this generalises to:\n",
    "\n",
    "$x_{n+1}=6^{o_{n}}(\\frac{x_0+\\sum_{i=0}^{i=n}{\\frac{2^{i+1}m_{i}}{6^{o_i}}})}{2^{n+1}})$\n",
    "\n",
    "Replacing $n$ with $n-1$ everywhere yields:\n",
    "\n",
    "$x_{n}=6^{o_{n-1}}(\\frac{x_0+\\sum_{i=0}^{i=n-1}{\\frac{2^{i+1}m_{i}}{6^{o_i}}})}{2^{n}})$\n",
    "\n",
    "### A simplifcation\n",
    "\n",
    "As beautiful identities go, this one needs some work:\n",
    "\n",
    "$x_{n}=6^{o_{n-1}}(\\frac{x_0+\\sum_{i=0}^{i=n-1}{\\frac{2^{i+1}m_{i}}{6^{o_i}}})}{2^{n}})$\n",
    "\n",
    "Recognising that $n-o_{n-1}$ = $e_{n-1}$ we get:\n",
    "\n",
    "$x_{n}=2^{o_{n-1}}3^{o_{n-1}}(\\frac{x_0+\\sum_{i=0}^{i=n-1}{\\frac{2^{i+1}m_{i}}{6^{o_i}}})}{2^{o_{n-1}+e_{n-1}}})$\n",
    "\n",
    "$x_{n}=\\frac{3^{o_{n-1}}{x_0+\\sum_{i=0}^{i=n-1}{\\frac{2^{i+1}3^{o_{n-1}}m_{i}}{2^{o_i}3^{o_i}}}}}{2^{e_{n-1}}}$\n",
    "\n",
    "$x_{n}=\\frac{3^{o_{n-1}}{x_0+\\sum_{i=0}^{i=n-1}{{2^{e_{i}}3^{o_{n-1}-o_i}m_{i}}}}}{2^{e_{n-1}}}$\n",
    "\n",
    "Rearranged, this yields:\n",
    "\n",
    "$k = 2^{e_{n-1}}x_{n}-3^{o_{n-1}}x_0=\\sum_{i=0}^{i=n-1}{{2^{e_{i}}3^{o_{n-1}-o_i}m_{i}}}$\n",
    "\n",
    "which describes an identity that applies to all Collatz sequences of finite length.\n",
    "\n",
    "A discussion about the structure of this identity and how this structure relates to the paths that are described is deferred to a future paper. For now, it is interesting to note, that $k$ is independent of $x_{0}$ and that all such paths of length $n+1$ which share the same sequence of odd-even transitions will have the same value of $k$."
   ]
  },
  {
   "cell_type": "markdown",
   "id": "a9243664",
   "metadata": {},
   "source": [
    "----\n",
    "$^*$ _whatever the importance of this contribution, the title is technically not wrong - these adjectives also describe paths that fail to reach their final objective_"
   ]
  },
  {
   "cell_type": "markdown",
   "id": "1c4405b8",
   "metadata": {},
   "source": [
    "# Appendix A: an example: $x_0=3 \\rightarrow x_7=1$\n",
    "\n",
    "Consider $x_0=3$:\n",
    "\n",
    "$\\{x_k\\} = \\{3, 10, 5, 16, 8, 4, 2, 1\\}$\n",
    "\n",
    "$n=7$\n",
    "\n",
    "$\\{m_k\\} = \\{1, 0, 1, 0, 0, 0, 0, 1\\}$\n",
    "\n",
    "$\\{o_k\\} = \\{1, 1, 2, 2, 2, 2, 2, 3\\}$\n",
    "\n",
    "$\\{e_k\\} = \\{0, 1, 1, 2, 3, 4, 5, 5\\}$\n",
    "\n",
    "The 8th term of $\\{x_k\\}$ is $x_7$=1.\n",
    "\n",
    "Substituting into the identity we have:\n",
    "\n",
    "$2^{e_6}x_{7} - 3^{o_6}x_0 = 2^{e_0}3^{o_6-o_0} +2^{e_2}3^{o_6-o_2}$\n",
    "\n",
    "$2^{e_6}x_{7} - 3^{o_6}x_0 = 2^{e_0}3^{o_6-o_0} +2^{e_2}3^{o_6-o_2}$\n",
    "\n",
    "$2^{5}x_{7} - 3^{2}x_0 = 2^{0}3^{2-1} +2^{1}3^{2-2}$\n",
    "\n",
    "$2^{5}x_{7} - 3^{2}x_0 = 2^{0}3^{1} +2^{1}3^{0}$\n",
    "\n",
    "$32x_{7} - 9x_0 = 3+2$\n",
    "\n",
    "$32\\times1 - 9\\times{3} = 3+2$\n",
    "\n",
    "$5 = 5$\n",
    "\n"
   ]
  },
  {
   "cell_type": "markdown",
   "id": "e70831bc",
   "metadata": {},
   "source": [
    "# Revision History\n",
    "    \n",
    "<div style=\"table {\n",
    "  float: left;\n",
    "}\">\n",
    "    \n",
    "|version|date|notes|\n",
    "|:--|:--|:--|\n",
    "|1.0.3|2023-10-14|cleanup some typos and added acknowledgments and dedications|\n",
    "|1.0.2|2023-10-14|a beautiful k formulation|\n",
    "|1.0.1|2023-10-12|slight cleanups of formulae.\n",
    "|1.0|12023-10-10|initial version - no revision history\n",
    "    \n",
    "</div>"
   ]
  },
  {
   "cell_type": "markdown",
   "id": "6f6ee8d4",
   "metadata": {},
   "source": [
    "# Acknowledgments\n",
    "\n",
    "There are many people who I would like to acknowledge for the support they have given me while writing this paper and at other times and so they will be when I receive their consent to be named by this paper."
   ]
  },
  {
   "cell_type": "markdown",
   "id": "0e8b7498",
   "metadata": {},
   "source": [
    "# Dedications\n",
    "\n",
    "This paper is dedicated to my parents, my sisters and their families in appreciation of their lifelong love and support and to Sonia for whom the following will always be true: non unum, duo aut tres. pax."
   ]
  }
 ],
 "metadata": {
  "kernelspec": {
   "display_name": "Python 3 (ipykernel)",
   "language": "python",
   "name": "python3"
  },
  "language_info": {
   "codemirror_mode": {
    "name": "ipython",
    "version": 3
   },
   "file_extension": ".py",
   "mimetype": "text/x-python",
   "name": "python",
   "nbconvert_exporter": "python",
   "pygments_lexer": "ipython3",
   "version": "3.11.5"
  }
 },
 "nbformat": 4,
 "nbformat_minor": 5
}
