{
 "cells": [
  {
   "cell_type": "markdown",
   "id": "b9b85b54",
   "metadata": {},
   "source": [
    "# A terminating, non-cyclic* path towards the Collatz conjecture\n",
    "\n",
    "Jon Seymour \\<a_beautiful_k\\@wildducktheories.com\\>\n",
    "\n",
    "14 October 2023\n",
    "\n",
    "## Abstract\n",
    "\n",
    "_\"Mathematics may not be ready for such problems\"_ - Paul ErdÅ‘s on the Collatz conjecture.\n",
    "\n",
    "It has long been known that the following identity applies to all paths of the Collatz sequence.\n",
    "\n",
    "$2^{e}x_{n} - 3^{o}x_{0} = k$\n",
    "\n",
    "where $x_{0}$ is the initial term and $x_{n}$ is the final term and $e$, $o$ and $k$ are path dependent parameters.\n",
    "\n",
    "This paper derives a formula for k derived from 3 parameter sequences $m_{n}, o_{n}, e_{n}$.\n",
    "\n",
    "$m_n = x_n\\pmod{2}$\n",
    "\n",
    "$o_{n} = \\sum_{k=0}^{k=n}{m_k}$\n",
    "\n",
    "$e_{n} = n+1 - o_{n}$\n",
    "\n",
    "$k_{n} = 2^{e_{n-1}}x_{n}-3^{o_{n-1}}x_0=\\sum_{i=0}^{i=n-1}{{2^{e_{i}}3^{o_{n-1}-o_i}m_{i}}}$\n",
    "\n",
    "The resultant identity is not novel, for example see \\[1\\], but perhaps the technique by which it was derived may be interesting to some.\n",
    "\n",
    "We also derive a recurrence relation that expresses each $k_{n}$ in terms of $k_{n-1}$\n",
    "\n",
    "$k_n = 3^{m_{n-1}}k_{n-1}+2^{e_{n-1}}m_{n-1}$\n",
    "\n",
    "and show that $k_{0} = 0$\n",
    "\n",
    "\n",
    "\\[1\\] [First odd term of the sequence lower odd number $n$ related to the $3\\cdot n+1$](https://mathoverflow.net/questions/448397/first-odd-term-of-the-sequence-lower-odd-number-n-related-to-the-3-cdot-n1?_gl=1*wy9ddp*_ga*MTAyNzkyMTgxNy4xNjYyNzY2MzQw*_ga_S812YQPLT2*MTY5NzI4NDUzNi40NS4xLjE2OTcyODUyMTMuMC4wLjA.) on [Maths Overflow Net](https://mathoverflow.net/)\n",
    "\n",
    "## A useful recurrence relation\n",
    "\n",
    "This paper examines a recurrence relation of the form:\n",
    "\n",
    "$x_{n+1} = \\frac{x_n+m_n(5x_n+2)}{2}, m_n=x_n\\pmod{2}$\n",
    "\n",
    "This sequence is identical to the known Collatz sequence, more traditionally defined as:\n",
    "\n",
    "$x_{n+1} = 3x_n + 1, x\\equiv1\\pmod{2}$\n",
    "\n",
    "$x_{n+1} = \\frac{x_n}{2}, x\\equiv0\\pmod{2}$\n",
    "\n",
    "That the relation is equivalent to the Collatz sequence is evident by re-arranging and simplifying this equation:\n",
    "\n",
    "$x_{n+1} = m_n(3x_n+1)+(1-m_n)\\frac{x}{2}$\n",
    "\n",
    "A single application of the recurrence relation can be represented as:\n",
    "\n",
    "$x_{n+1}=succ^{(1)}(x_n)$\n",
    "\n",
    "k-repeated applications of the recurrence relation can be represented thus:\n",
    "\n",
    "$x_{n+k}=succ^{(k)}(x_n)$\n",
    "\n",
    "Alternatively, $x_n$, can be expressed, for some $n$ and $x_0$, thus:\n",
    "\n",
    "$x_{n}=succ^{(n)}(x_0)$\n",
    "\n",
    "## Alternative forms of the recurrence relation\n",
    "\n",
    "Using the identity: \n",
    "\n",
    "$5m+1 = 6^m = 2^m3^m \\iff {m}\\in\\{0,1\\}$ \n",
    "\n",
    "the same recurrence relation can also be expressed in all of the following ways:\n",
    "\n",
    "$x_{n+1} = \\frac{(5m_n+1)x_n+2m_n}{2}$\n",
    "\n",
    "$x_{n+1} = \\frac{6^{m_n}x_n+2m_n}{2}$\n",
    "\n",
    "$x_{n+1} = \\frac{2^{m_n}3^{m_n}x_n+2m_n}{2}$\n",
    "\n",
    "$x_{n+1} = 2^{{m_n}-1}3^{m_n}x_n+m_n$\n",
    "\n",
    "and, finally, this:\n",
    "\n",
    "$x_{n+1} = 2^{{m_n}-1}((2+1)^{m_n}x_n+m_n)$\n",
    "\n",
    "in which $3^{m_n}$ been replaced by $({2+1})^{m_n}$\n",
    "\n"
   ]
  },
  {
   "cell_type": "code",
   "execution_count": null,
   "id": "085cafe5",
   "metadata": {},
   "outputs": [],
   "source": [
    "from fractions import Fraction\n",
    "import math\n",
    "\n",
    "def m(x):\n",
    "    return x%2\n",
    "\n",
    "def succ(x):\n",
    "    succ=(x+m(x)*(5*x+2))//2\n",
    "    assert not(x%2 == 0) or succ == x//2\n",
    "    assert not(x%2 == 1) or succ == 3*x+1\n",
    "    assert succ == (6**(m(x))*x+2*m(x))//2\n",
    "    assert succ == (2**(m(x))*3**(m(x))*x+2*m(x))//2\n",
    "    assert succ == 2**(m(x)-1)*3**(m(x))*x+m(x)\n",
    "    assert succ == 2**(m(x)-1)*(2+1)**(m(x))*x+m(x)\n",
    "    return succ\n",
    "\n",
    "def collatz(x0, n):\n",
    "    x=x0\n",
    "    for k in range(0, n):\n",
    "        yield {\"i\": k, \"x\": x, \"x0\": x0, \"m\": m(x), \"succ\": succ(x)}    \n",
    "        x=succ(x)\n",
    "\n",
    "result=[e for e in collatz(27, 10)]\n",
    "#result"
   ]
  },
  {
   "cell_type": "markdown",
   "id": "56c3b852",
   "metadata": {},
   "source": [
    "## The sequences $o_{n}$, $e_{n}$\n",
    "\n",
    "Let $o_{0} = m_0, o_{n+1} = o_{n}+m_{n+1}, n>0$.\n",
    "\n",
    "Let $e_{n} = {n+1}-o_{n}$\n",
    "\n",
    "Clearly:\n",
    "\n",
    "$o_{n} = \\sum_{k=0}^{k=n}{m_k}$\n",
    "\n",
    "$e_{n} = \\sum_{k=0}^{k=n}(1-{m_k})$\n",
    "\n",
    "### Interpretation\n",
    "\n",
    "The series $o_{n}$ and $e_{n}$ is that they represent the number of odd and even terms in the path between $x_0$ and $x_n$. "
   ]
  },
  {
   "cell_type": "code",
   "execution_count": null,
   "id": "312562df",
   "metadata": {},
   "outputs": [],
   "source": [
    "def o(seq):\n",
    "    for e in seq:\n",
    "        if e[\"i\"] == 0:\n",
    "            e[\"o\"]=e[\"m\"]\n",
    "        else:\n",
    "            e[\"o\"]=pred[\"o\"]+e[\"m\"]            \n",
    "        assert e[\"o\"] <= e[\"i\"]+1\n",
    "        yield e\n",
    "        pred=e\n",
    "        \n",
    "def e(seq):\n",
    "    for e in o(seq):\n",
    "        e[\"e\"]=e[\"i\"]+1-e[\"o\"]\n",
    "        assert e[\"o\"]+e[\"e\"]==e[\"i\"]+1\n",
    "        yield e\n",
    "        \n",
    "result=[e for e in e(collatz(27, 10))]\n",
    "#result"
   ]
  },
  {
   "cell_type": "markdown",
   "id": "950c4f4e",
   "metadata": {},
   "source": [
    "## An expression for $x_{n}$ in terms of $x_{0}$.\n",
    "\n",
    "### the sequences $a_{n}$, $c_{n}$ and $d_{n}$\n",
    "\n",
    "In this section we rewrite each term $x_{n}$ as combination of terms from\n",
    "three simpler monotonically incresing sequences: \n",
    "- $a_{n}$ (_the accumulator sequence_)\n",
    "- $c_{n}$ (_the coefficient sequence_)\n",
    "- $d_{n}$ (_the divisor sequence_).\n",
    "\n",
    "Let the first term of the sequence, $x_{n}$ be named $x_{0}$ with subsequent terms being $x_{1}, x_{2}$ et cetera.\n",
    "\n",
    "Then we can define:\n",
    "\n",
    "$x_{n}=\\frac{c_{n}x_{0}+a_{n}}{d_{n}}$\n",
    "\n",
    "with $a_{0}=0$, $c_{0}=1$ and $d_{0}=1$.\n",
    "\n",
    "Now, let's derive an expression for $x_{n+1}$ in terms of $x_{0}, a_{n}, c_{n}$ and $d_{n}$\n",
    "\n",
    "Recall that:\n",
    "\n",
    "$x_{n+1} = \\frac{x_n+m_n(5x_n+2)}{2}$\n",
    "\n",
    "Substituting $\\frac{c_{n}x_{0}+a_{n}}{d_{n}}$ for $x_n$ yields:\n",
    "\n",
    "$x_{n+1} = \\frac{\\frac{c_{n}x_{0}+a_{n}}{d_{n}}+m_n(5(\\frac{c_{n}x_{0}+a_{n}}{d_{n}})+2)}{2}$\n",
    "\n",
    "Simplifying:\n",
    "\n",
    "$x_{n+1} = \\frac{{c_{n}x_{0}+a_{n}}+m_n(5({c_{n}x_{0}+a_{n}})+2d_{n})}{2d_{n}}$\n",
    "\n",
    "Redistributing terms:\n",
    "\n",
    "$x_{n+1}=\\frac{{c_{n}(5m_{n}+1)x_{0}+a_{n}(5m_{n}+1)}+m_n2d_{n}}{2d_{n}}$\n",
    "\n",
    "Noting the identity:\n",
    "\n",
    "$5m_{n}+1 = 6^{m_n}$\n",
    "\n",
    "$a_n$ can be further simplified to:\n",
    "\n",
    "$x_{n+1}=\\frac{6^{m_n}{c_{n}x_{0}+6^{m_n}a_{n}}+m_n2d_{n}}{2d_{n}}$\n",
    "\n",
    "This is of the form:\n",
    "\n",
    "$x_{n+1}=\\frac{c_{n+1}x_{0}+a_{n+1}}{d_{n+1}}$\n",
    "\n",
    "with:\n",
    "\n",
    "$a_{n+1}=6^{m_n}a_{n}+m_{n}2d_{n}$\n",
    "\n",
    "$c_{n+1}=6^{m_n}c_{n}$\n",
    "\n",
    "$d_{n+1}=2d_{n}$"
   ]
  },
  {
   "cell_type": "code",
   "execution_count": null,
   "id": "766423bb",
   "metadata": {},
   "outputs": [],
   "source": [
    "def d(seq):\n",
    "    for e in seq:\n",
    "        if e[\"i\"] == 0:\n",
    "            e[\"d\"]=1\n",
    "        else:\n",
    "            e[\"d\"]=(2*pred[\"d\"])\n",
    "        yield e\n",
    "        pred=e\n",
    "\n",
    "def c(seq):\n",
    "    for e in seq:\n",
    "        if e[\"i\"] == 0:\n",
    "            e[\"c\"]=1\n",
    "        else:\n",
    "            e[\"c\"]=(6**pred[\"m\"])*pred[\"c\"]\n",
    "        yield e\n",
    "        pred=e\n",
    "\n",
    "def a(seq):\n",
    "    for e in d(seq):\n",
    "        if e[\"i\"] == 0:\n",
    "            e[\"a\"]=0\n",
    "        else:\n",
    "            e[\"a\"]=(6**pred[\"m\"])*pred[\"a\"]+(2*pred[\"m\"]*pred[\"d\"])\n",
    "        yield e\n",
    "        pred=e\n",
    "                                             \n",
    "def a_c_d(seq):\n",
    "    for e in c(a(seq)):\n",
    "        if e[\"i\"] > 0:\n",
    "            assert e[\"x\"] == (e[\"c\"]*e[\"x0\"]+e[\"a\"])/e[\"d\"]\n",
    "        yield e\n",
    "        pred=e                                    \n",
    "                                                 \n",
    "\n",
    "results=[e for e in a_c_d(collatz(27, 10))]\n",
    "#results"
   ]
  },
  {
   "cell_type": "markdown",
   "id": "50c379c3",
   "metadata": {},
   "source": [
    "## Rewriting $a_{n+1}$, $c_{n+1}$, $d_{n+1}$, $x_{n+1}$ in terms of $x_0$\n",
    "\n",
    "### Case: $x_0 \\rightarrow x_1$\n",
    "\n",
    "We can check this for n=0 as follows:\n",
    "\n",
    "$a_{1}=6^{m_0}a_{0}+2m_{0}d_{0}=2m_{0}d_{0}=2m_{0}$\n",
    "\n",
    "$c_{1}=6^{m_0}c_{0}=6^{m_0}$\n",
    "\n",
    "$d_{1}=2d_{0}=2$\n",
    "\n",
    "$x_{1}=\\frac{6^{m_0}x_{0}+2m_{0}}{2} = \\frac{({5m_{0}+2}){x_0}+m_{0}}{2} = \\frac{x_{0} + m_{0}(5x_{0}+2)}{2} = succ^{(1)}(x_0)$\n",
    "\n",
    "### Case: $x_0 \\rightarrow x_1 \\rightarrow x_2$\n",
    "\n",
    "$a_{2}=6^{m_1}a_{1}+2d_{1}m_{1} = 6^{m_1}m_{0}2+m_{1}4$\n",
    "\n",
    "$c_{2}=6^{m_1}c_{1}=6^{m_1}6^{m_0}$\n",
    "\n",
    "$d_{2}=2d_{1} = 4$\n",
    "\n",
    "$x_{2}=\\frac{6^{m_1}6^{m_0}x_{0}+6^{m_1}m_{0}2+m_{1}4}{4} = succ^{(2)}(x_0)$\n",
    "\n",
    "### Case: $x_0 \\rightarrow x_1 \\rightarrow x_2 \\rightarrow x_3$\n",
    "\n",
    "$a_{3}=6^{m_2}a_{2}+2d_{2}m_{2}=6^{m_2}(6^{m_1}2m_{0}+4m_{1})+m_{2}8=6^{m_2}6^{m_1}m_{0}2+6^{m_2}m_{1}4+m_{2}8$\n",
    "\n",
    "$a_{3} = 6^{o_2}(\\sum_{i=0}^{i=2}{\\frac{2^{i+1}m_{i}}{6^{o_i}}})$\n",
    "\n",
    "$c_{3}=6^{m_2}6^{m_1}6^{m_0}=6^{o_{2}}$\n",
    "\n",
    "$d_{3}=8=2^3$\n",
    "\n",
    "$x_{3}=\\frac{6^{o_{2}}x_0+6^{o_2}(\\sum_{i=0}^{i=2}{\\frac{2^{i+1}m_{i}}{6^{o_i}}})}{2^3}$\n",
    "\n",
    "$x_{3}=6^{o_{2}}(\\frac{x_0+\\sum_{i=0}^{i=2}{\\frac{2^{i+1}m_{i}}{6^{o_i}}})}{2^3}) = succ^{(3)}(x_0)$\n",
    "\n",
    "### Case: $x_0 \\rightarrow \\ldots \\rightarrow x_n \\rightarrow x_{n+1}$\n",
    "\n",
    "It can be shown that this generalises to:\n",
    "\n",
    "$x_{n+1}=6^{o_{n}}(\\frac{x_0+\\sum_{i=0}^{i=n}{\\frac{2^{i+1}m_{i}}{^{o_i}}}}{2^{n+1}})$\n",
    "\n",
    "Replacing $n$ with $n-1$ everywhere yields:\n",
    "\n",
    "$x_{n}=6^{o_{n-1}}(\\frac{x_0+\\sum_{i=0}^{i=n-1}{\\frac{2^{i+1}m_{i}}{6^{o_i}}}}{2^{n}})$\n",
    "\n",
    "$x_{n}=6^{o_{n-1}}(\\frac{x_0+\\sum_{i=0}^{i=n-1}{\\frac{2^{i+1}m_{i}}{6^{o_i}}}}{2^{n}})$\n",
    "\n",
    "Recognising that $n-o_{n-1}$ = $e_{n-1}$ we get:\n",
    "\n",
    "$x_{n}=2^{o_{n-1}}3^{o_{n-1}}(\\frac{x_0+\\sum_{i=0}^{i=n-1}{\\frac{2^{i+1}m_{i}}{2^{o_i}3^{o_i}}}}{2^{o_{n-1}+e_{n-1}}})$\n",
    "\n",
    "$x_{n}=\\frac{3^{o_{n-1}}({x_0+\\sum_{i=0}^{i=n-1}{\\frac{2^{e_i}m_{i}}{3^{o_i}}}})}{2^{e_{n-1}}}$\n",
    "\n",
    "$x_{n}=\\frac{3^{o_{n-1}}}{2^{e_{n-1}}}({x_0+\\sum_{i=0}^{i=n-1}{\\frac{2^{e_i}m_{i}}{3^{o_i}}}})=succ^{(n)}(x_0)$\n",
    "\n",
    "\n",
    "## A Beautiful $k$\n",
    "\n",
    "Re-arranged, the expression for $x_{n}$ yields an expression for $k_{n}$ the value of $2^{e_{n-1}}x_{n}-3^{o_{n-1}}x_0$\n",
    "\n",
    "$k_n = 2^{e_{n-1}}x_{n}-3^{o_{n-1}}x_0=3^{o_{n-1}}\\sum_{i=0}^{i=n-1}{}\\frac{2^{e_{i}}}{3^{o_i}}m_{i}$\n",
    "\n",
    "which describes an identity that applies to all Collatz sequences of finite length.\n",
    "\n",
    "We refer to this as _the beautiful k_ because rather than being an opaque, structure-less $k$, the formula\n",
    "captures, in a single expression, the intricate twists and turns of any particular Collatz sequence with a simple\n",
    "expression involving only a scaling factor, $3^{o_{n-1}}$ and a series that includes a term, $\\frac{2^{e_{i}}}{3^{o_i}}m_{i}$ for each term in the underlying sequence, scaled according to its position in the sequence. Only \n",
    "the odd series terms contribute directly to the final sum, but even the even series terms make their presence felt\n",
    "by scaling the subsequent odd terms via the $2^{e_i}$ exponents.\n",
    "\n",
    "## The sequence $k_n$\n",
    "\n",
    "This section we derive an expression $k_n$ in terms of $k_{n-1}$ the identity that relates $x_{0}$ and $x_{n-1}$.\n",
    "\n",
    "$k_n = 3^{m_{n-1}+o_{n-2}}(\\sum_{i=0}^{i=n-2}{}\\frac{2^{e_{i}}}{3^{o_i}}m_{i}+\\frac{2^{e_{n-1}}}{3^{o_{n-1}}}m_{n-1})$\n",
    "\n",
    "$k_n = 3^{m_{n-1}}(k_{n-1}+3^{o_{n-2}}\\frac{2^{e_{n-1}}}{3^{o_{n-1}}}m_{n-1})$\n",
    "\n",
    "$k_n = 3^{m_{n-1}}k_{n-1}+2^{e_{n-1}}m_{n-1}$\n",
    "\n",
    "To be well-defined for n, we need an expression for $k_{0}$.\n",
    "\n",
    "Subtituting $n=1$ we get:\n",
    "\n",
    "$k_1 = 3^{m_0}k_{0}+2^{e_{0}}m_{0}$\n",
    "\n",
    "but we also know:\n",
    "\n",
    "$k_1 = 2^{e_0}x_{1}-3^{o_0}x_0$\n",
    "\n",
    "So:\n",
    "\n",
    "$3^{m_0}k_{0}+2^{e_{0}}m_{0} = 2^{e_0}x_{1}-3^{o_0}x_0$\n",
    "\n",
    "Re-arranged:\n",
    "\n",
    "$k_{0} = \\frac{2^{e_0}(x_{1}-m_{0})}{3^{m_0}}-x_0$\n",
    "\n",
    "Substituting:\n",
    "\n",
    "$x_{1} = \\frac{6^{m_0}x_0+2m_0}{2}$\n",
    "\n",
    "$k_{0} = \\frac{2^{e_0}({\\frac{6^{m_0}x_0+2m_0}{2}}-m_{0})}{3^{m_0}}-x_0$\n",
    "\n",
    "$k_{0} = \\frac{2^{{e_0}-1}({6^{m_0}x_0+2m_0}-2m_{0})}{3^{m_0}}-x_0$\n",
    "\n",
    "Simplifying:\n",
    "\n",
    "$k_{0} = {2^{e_0+m_{0}-1}x_0}-x_0=(2^{e_0+m_{0}-1}-1)x_0$\n",
    "\n",
    "But $e_0=1-o_{0}$, $o_{0}=m_{0}, e_{0}+o_{0}-1 = 0$ so:\n",
    "\n",
    "$k_{0} = (2^0-1)x_0 = (1-1)x_0 = (0)x_0 = 0$\n",
    "\n",
    "So:\n",
    "\n",
    "$k_n = 3^{m_{n-1}}k_{n-1}+2^{e_{n-1}}m_{n-1}, n>0$\n",
    "\n",
    "$k_0 = 0, n=0$\n",
    "\n",
    "We note that:\n",
    "\n",
    "- $m_{n-1} = 0 \\iff k_{n}=k_{n-1}$\n",
    "- $m_{n-1} = 1 \\iff k_{n}=3k_{n-1}+2^{e_{n-1}}$\n",
    "- $k_{n} >= k_{n-1}$"
   ]
  },
  {
   "cell_type": "code",
   "execution_count": null,
   "id": "541a2ccd",
   "metadata": {},
   "outputs": [],
   "source": [
    "def k(seq):\n",
    "    for e_ in e(seq):\n",
    "        if e_[\"i\"] == 0:\n",
    "            e_[\"k\"] = 0\n",
    "        else:\n",
    "            e_[\"k\"]=(3**pred[\"m\"])*pred[\"k\"]+(2**pred[\"e\"])*pred[\"m\"]\n",
    "            assert (2**pred[\"e\"])*e_[\"x\"]-(3**pred[\"o\"])*e_[\"x0\"] == e_[\"k\"]\n",
    "        yield e_\n",
    "        pred=e_\n",
    "\n",
    "results=[e for e in k(collatz(27, 112))]\n",
    "#results"
   ]
  },
  {
   "cell_type": "markdown",
   "id": "4625fb1b",
   "metadata": {},
   "source": [
    "## Definition: $u, x_{u}$\n",
    "\n",
    "Recall that:\n",
    "\n",
    "$x_n=succ^{(n)}(x_0)$\n",
    "\n",
    "Now define $u$ be the smallest value of $n$ such that $x_n = x_u = succ^{(u)}(x_0) = 1$, if such a value\n",
    "exists and to be undefined otherwise."
   ]
  },
  {
   "cell_type": "markdown",
   "id": "d1737f90",
   "metadata": {},
   "source": [
    "## An expression for $x_0$ in terms of $\\{i\\in[0,n-1]: m_i\\}$\n",
    "\n",
    "In the final analysis, an expression for $k$ is only useful if it leads to progress towards the Collatz conjecture:\n",
    "\n",
    "Now let's forget $k$, and consider the identity:\n",
    "\n",
    "$2^{e_{n-1}}x_{n}-3^{o_{n-1}}x_0=3^{o_{n-1}}\\sum_{i=0}^{i=n-1}{{\\frac{2^{e_{i}}}{3^{o_i}}}m_{i}}$\n",
    "\n",
    "Let's assume that the conjecture is true. Given the identity holds and substituting $x_n=x_u=1$ then:\n",
    "\n",
    "$\\text{Collatz} \\implies \\forall x_0\\in\\mathbb{N}: \\exists{u\\in\\mathbb{N}, m_{i}\\in[0,1]}: 2^{e_{u-1}}-3^{o_{u-1}}x_0=3^{o_{u-1}}\\sum_{i=0}^{i=u-1}{{\\frac{2^{e_{i}}}{3^{o_i}}}m_{i}}$\n",
    "\n",
    "Rearranging and factoring out common terms we get:\n",
    "\n",
    "$2^{e_{u-1}}=3^{o_{n-1}}(x_0 + \\sum_{i=0}^{i=u-1}$ $\\frac{{2^{e_{i}}m_i}}{{3^{o_{i}}}})$\n",
    "\n",
    "Solving for ${x_0}$ we get:\n",
    "\n",
    "$\\text{Collatz} \\implies \\forall x_0\\in\\mathbb{N}: \\exists{u\\in\\mathbb{N}, m_{i}\\in[0,1]}: x_0 = \\frac{2^{e_{u-1}}}{3^{o_{u-1}}} - \\sum_{i=0}^{i=u-1}$ $\\frac{{2^{e_{i}}m_{i}}}{{3^{o_{i}}}}$"
   ]
  },
  {
   "cell_type": "markdown",
   "id": "a24512f4",
   "metadata": {},
   "source": [
    "## Congruency of paths\n",
    "\n",
    "Two Collatz sequences of the same length are congruent if, and only if, their identities are equal, that is:\n",
    "\n",
    "${x_0\\ldots{x_n}}\\cong{y_0\\ldots{y_n}}\\iff{2^{e_{n-1}}x_{n}-3^{o_{n-1}}x_0}={2^{e_{n-1}}y_{n}-3^{o_{n-1}}y_0}=3^{o_{n-1}}\\sum_{i=0}^{i=n-1}{{\\frac{2^{e_{i}}}{3^{o_i}}}m_{i}}$\n",
    "\n",
    "By definition, two paths are in the same congruency class if, and only if, they are congruent by the defintion above.\n",
    "\n",
    "## Path class identifiers\n",
    "\n",
    "Let $p_{n,k}$ be defined as:\n",
    "\n",
    "$p_{n,k}: 2^\\mathbb{N}\\rightarrow\\mathbb{N}: 2^n+\\sum_{i=0}^{i=n-1}{2^i}{m_{i}}$\n",
    "\n",
    "$p_{n,k}$ can be interpreted as identifier of the class of paths of length $n+1$ which are congruent to $k$.\n",
    "\n",
    "The isolated $2^n$ term serves to encode the length of the path and thus helps to distinguish the class path identifiers for paths like $8\\rightarrow{4}\\rightarrow{2}\\text{ (1000) and }4\\rightarrow{2}\\text{ (100)}$."
   ]
  },
  {
   "cell_type": "markdown",
   "id": "75a04ca6",
   "metadata": {},
   "source": [
    "----\n",
    "$^*$ _whatever the importance of this contribution, the title is technically not wrong - these adjectives also describe paths that fail to reach their final objective_"
   ]
  },
  {
   "cell_type": "markdown",
   "id": "1c4405b8",
   "metadata": {},
   "source": [
    "# Appendix A: an example: $x_0=3 \\rightarrow x_7=1$\n",
    "\n",
    "Consider $x_0=3$:\n",
    "\n",
    "$\\{x_k\\} = \\{3, 10, 5, 16, 8, 4, 2, 1\\}$\n",
    "\n",
    "$n=7$\n",
    "\n",
    "$\\{m_k\\} = \\{1, 0, 1, 0, 0, 0, 0, 1\\}$\n",
    "\n",
    "$\\{o_k\\} = \\{1, 1, 2, 2, 2, 2, 2, 3\\}$\n",
    "\n",
    "$\\{e_k\\} = \\{0, 1, 1, 2, 3, 4, 5, 5\\}$\n",
    "\n",
    "The 8th term of $\\{x_k\\}$ is $x_7$=1.\n",
    "\n",
    "Substituting into the identity we have:\n",
    "\n",
    "$2^{e_6}x_{7} - 3^{o_6}x_0 = 2^{e_0}3^{o_6-o_0} +2^{e_2}3^{o_6-o_2}$\n",
    "\n",
    "$2^{e_6}x_{7} - 3^{o_6}x_0 = 2^{e_0}3^{o_6-o_0} +2^{e_2}3^{o_6-o_2}$\n",
    "\n",
    "$2^{5}x_{7} - 3^{2}x_0 = 2^{0}3^{2-1} +2^{1}3^{2-2}$\n",
    "\n",
    "$2^{5}x_{7} - 3^{2}x_0 = 2^{0}3^{1} +2^{1}3^{0}$\n",
    "\n",
    "$32x_{7} - 9x_0 = 3+2$\n",
    "\n",
    "$32\\times1 - 9\\times{3} = 3+2$\n",
    "\n",
    "$5 = 5$\n",
    "\n"
   ]
  },
  {
   "cell_type": "markdown",
   "id": "e70831bc",
   "metadata": {},
   "source": [
    "# Revision History\n",
    "    \n",
    "|version|date|notes|\n",
    "|:--|:--|:--|\n",
    "|1.0.5|2023-10-14|fixed alternative recurrence relations - thanks A! Added notes about path congruency and path class identifiers, notes about identity if Conjecture is true. Added expressions for the sequence $k_n$. Defined $u$, $x_u$. Corrected deriviations of $a_n, c_n, d_n$. Provided implementations of $a_{n},c_{n},d_{n},e_{n}$ and $k_{n}$|\n",
    "|1.0.4|2023-10-14|reworded abstract to reflect the fact the identity is already well known|\n",
    "|1.0.3|2023-10-14|cleanup some typos and added acknowledgments and dedications|\n",
    "|1.0.2|2023-10-14|a beautiful k formulation|\n",
    "|1.0.1|2023-10-12|slight cleanups of formulae.\n",
    "|1.0|12023-10-10|initial version - no revision history"
   ]
  }
 ],
 "metadata": {
  "kernelspec": {
   "display_name": "Python 3 (ipykernel)",
   "language": "python",
   "name": "python3"
  },
  "language_info": {
   "codemirror_mode": {
    "name": "ipython",
    "version": 3
   },
   "file_extension": ".py",
   "mimetype": "text/x-python",
   "name": "python",
   "nbconvert_exporter": "python",
   "pygments_lexer": "ipython3",
   "version": "3.11.5"
  }
 },
 "nbformat": 4,
 "nbformat_minor": 5
}
